Always eventually big push

examples/Queue.v
@@ -4,6 +4,7 @@ From CTree Require Import
   Logic.Ctl
   CTree.Equ
   CTree.SBisim
+  CTree.Logic.Trans
   CTree.Logic.AX
   CTree.Logic.AF
   CTree.Logic.Bind
@@ -53,14 +54,14 @@ Arguments push /.
 Arguments pop /.
 
 Section QueueEx.
-  Context {S: Type} {HDec: RelDec (@eq S)} {HCor: RelDec_Correct HDec}.
+  Context {T: Type} {HDec: RelDec (@eq T)} {HCor: RelDec_Correct HDec}.
   Infix "=?" := (rel_dec) (at level 75).
 
   (* Queue instrumented semantics *)
-  Definition h_queueE: queueE S ~> stateT (list S) (ctreeW S) := 
+  Definition h_queueE: queueE T ~> stateT (list T) (ctreeW T) := 
     fun e =>
       mkStateT (fun q =>
-                 match e return ctreeW S (encode e * list S) with
+                 match e return ctreeW T (encode e * list T) with
                  | Push v => Ret (tt, q ++ [v])
                  | Pop => match q with
                          | nil => Ret (None, nil)
@@ -71,7 +72,7 @@ Section QueueEx.
                  end).
   
   (* Ex1: Drain a queue until there is nothing left, you should get a needle in the end eventually. *)
-  Definition drain: ctree (queueE S) unit :=
+  Definition drain: ctree (queueE T) unit :=
     iter (fun _ =>
             x <- pop ;;
             match x with
@@ -79,11 +80,11 @@ Section QueueEx.
             | None => Ret (inr tt)   (* done *)
             end) tt.        
 
-  Lemma list_app_nil: forall (s: S) hs,
+  Lemma list_app_nil: forall (s: T) hs,
       ~ [] = hs ++ [s].  
   Proof. destruct hs; intros * H; inv H; auto. Qed.
 
-  Lemma list_app_cons: forall (h s: S) ts hs,
+  Lemma list_app_cons: forall (h s: T) ts hs,
       h :: ts = hs ++ [s] ->
       match hs with
       | nil => h = s /\ ts = nil
@@ -93,14 +94,14 @@ Section QueueEx.
     
   (*| Eventually we get [nl] (needle) to show up
     in the instrumentation. |*)
-  Example drain_af_pop: forall (nl: S) (q: list S),
+  Example drain_af_pop: forall (nl: T) (q: list T),
       <[ {interp_state h_queueE drain (q ++ [nl])}, Pure |=
-         AF finishW {fun 'tt l w => w = nl /\ l = @nil S }]>.
+         AF finishW {fun 'tt l w => w = nl /\ l = [] }]>.
   Proof with eauto with ctl.    
     intros.
     apply aur_state_iter_nat
       with (f:=fun 'tt l _ => List.length l)
-           (Ri:=fun 'tt l w => not_done w /\
+           (Ri:=fun 'tt l w => 
                   match w with
                   | Obs (Log s') tt =>
                       match l with
@@ -109,7 +110,7 @@ Section QueueEx.
                       end
                   | _ => exists hs, l = hs ++ [nl]
                   end)... 
-    intros [] l w (Hd & Hw).
+    intros [] l w Hd Hw.
     destruct l as [|h ts] eqn:Hl; subst.
     - (* l = [] *)
       inv Hd.
@@ -165,108 +166,378 @@ Section QueueEx.
       + cbn.
         rewrite interp_state_ret.
         cleft.        
-        apply anr_ret; [constructor |split;[split; cbn|]]...
-        inv Hd.
-        * destruct Hw.
-          apply list_app_cons in H.
-          destruct x; intuition; subst...
-          destruct x; intuition; cbn.
-          ++ now (exists []).
-          ++ now (exists (s0 ::x)).
-        * destruct e, v, Hw.
-          apply list_app_cons in H.
-          destruct x; intuition; subst...
-          destruct x; intuition; cbn.
-          ++ now (exists []).
-          ++ now (exists (s1 ::x)).
+        apply anr_ret; [constructor |split]...
+        split.
+        * inv Hd.
+          -- destruct Hw.
+             apply list_app_cons in H.
+             destruct x; intuition; subst...
+             destruct x; intuition; cbn.
+             ++ now (exists []).
+             ++ now (exists (t0 ::x)).
+          -- destruct e, v, Hw.
+             apply list_app_cons in H.
+             destruct x; intuition; subst...
+             destruct x; intuition; cbn.
+             ++ now (exists []).
+             ++ now (exists (t1 ::x)).
+        * apply PeanoNat.Nat.lt_succ_diag_r.
   Qed.
-
-  Definition while{E} `{HE: Encode E}(k: ctree E (unit + unit)): ctree E unit :=
-    Ctree.iter (fun _ => k tt) tt.
   
   (* Ex2: Rotate a queue (pop an element from head, add it to tail) *)
-  Definition rotate: ctree (queueE S) unit :=
-    iter (fun _ =>
-            x <- pop ;;
-            match x with
-            | Some v =>
-                push v;;
-                Ret (inl tt)
-            | None =>
-                (* If queue is empty to begin with, return [tt] *)
-                Ret (inr tt)
-            end) tt.
-  
-  Inductive index: list S -> S -> nat -> Prop :=
-  | IndexFound: forall h h' ts,
-      h = h' ->
-      index (h :: ts) h' 0
-  | IndexSucc: forall h ts x n,
-    index ts x n ->
-    index (h :: ts) x (1+ n)%nat.
-  Hint Constructors index: core.
+  Definition rotate: ctree (queueE T) void :=
+    Ctree.forever void (fun _ =>
+                          x <- pop ;;
+                          match x with
+                          | Some v =>
+                              push v;;
+                              Ret tt
+                          | None => Ret tt
+                          end) tt.
 
-  Lemma index_last_eq: forall q (nl: S),
-      index (q ++ [nl]) nl (length q).
+  (* Element [t] does not appear in [l] *)
+  Fixpoint not_inb(t: T)(l: list T): bool :=
+    match l with
+    | nil => true
+    | h :: ts =>
+        if h =? t then
+          false
+        else
+          not_inb t ts
+    end.
+
+  (* Element [t] appears unique in [l] in some position *)
+  Fixpoint unique(t: T) (l: list T): option nat :=
+    match l with
+    | nil => None
+    | h :: ts => if h =? t then
+                 if not_inb t ts then
+                   Some 0
+                 else
+                   None
+               else
+                 option_map S (unique t ts)
+    end.
+
+  Fixpoint last_error(l: list T): option T :=
+    match l with
+    | nil => None
+    | v :: nil => Some v
+    | _ :: ts => last_error ts
+    end.
+  
+  Lemma unfold_unique_hd: forall t h ts,
+      unique t (h :: ts) =
+        (if h =? t then
+                 if not_inb t ts then
+                   Some 0
+                 else
+                   None
+               else
+                 option_map S (unique t ts)).
+  Proof.
+    reflexivity.
+  Qed.
+  
+  Lemma unique_head_eq': forall nl q,
+      not_inb nl q = true ->
+      unique nl (nl :: q) = Some 0.
   Proof with auto.
-    induction q; intros; cbn; auto.
+    intros; cbn.
+    rewrite rel_dec_eq_true...
+    now rewrite H.
+  Qed.
+  
+  Lemma unique_head_eq: forall nl t q i,      
+      unique nl (t :: q) = Some i ->
+      (t =? nl) = true ->
+      not_inb nl q = true.
+  Proof.
+    intros.
+    cbn in H.
+    rewrite H0 in H.
+    destruct (not_inb nl q); inv H.
+    reflexivity.
   Qed.
 
+  Lemma unique_head_neq': forall nl t q i,
+      (t =? nl) = false ->
+      unique nl q = Some i ->
+      unique nl (t :: q) = Some (S i).
+  Proof.
+    intros.
+    cbn.
+    rewrite H, H0.
+    reflexivity.
+  Qed.
+  
+  Lemma unique_head_neq: forall nl t q i,
+      unique nl (t :: q) = Some i ->
+      (t =? nl) = false ->      
+      unique nl q = Some (i - 1).
+  Proof.
+    induction q; cbn; intros;
+      rewrite H0 in *.
+    inv H.
+    destruct (a =? nl) eqn:Ha.
+    - apply rel_dec_correct in Ha; subst.
+      destruct (not_inb nl q); inv H.
+      reflexivity. 
+    - destruct (unique nl q) eqn:Hnl; cbn in *; inv H.
+      rewrite H0 in IHq.
+      reflexivity.
+  Qed.
+  
+  Lemma unique_last_eq: forall q nl,
+      not_inb nl q = true ->
+      unique nl (q ++ [nl]) = Some (List.length q).
+  Proof with auto.
+    induction q; cbn; intros.
+    - rewrite rel_dec_eq_true...
+    - destruct (a =? nl); inv H.
+      rewrite IHq...
+  Qed.
+
+  Lemma not_inb_last_false: forall q nl,
+      not_inb nl (q ++ [nl]) = false.
+  Proof with auto.
+    induction q; cbn; intros.
+    - rewrite rel_dec_eq_true...
+    - destruct (a =? nl)...
+  Qed.
+  
+  Lemma unique_last_none: forall q nl i,
+      unique nl q = Some i ->
+      unique nl (q ++ [nl]) = None.
+  Proof with auto.
+    induction q; cbn; intros.
+    - inv H.
+    - destruct (a =? nl) eqn:Hnl, (not_inb nl q) eqn:Hin; inv H.
+      + rewrite not_inb_last_false...
+      + destruct (unique nl q) eqn:Hnl'; inv H1.
+        erewrite IHq with (i:=n)...
+      + destruct (unique nl q) eqn:Hnl'; inv H1.
+        erewrite IHq with (i:=n)...
+  Qed.
+  
+  Lemma not_inb_unique_none: forall q nl,
+      not_inb nl q = true ->
+      unique nl q = None.
+  Proof with auto.
+    induction q; intros; cbn...
+    cbn in H.
+    destruct (a =? nl); inv H.
+    rewrite IHq...
+  Qed.
+
+  Lemma not_inb_app_true: forall nl q q',
+      not_inb nl q = true ->
+      not_inb nl q' = true ->
+      not_inb nl (q ++ q') = true.
+  Proof with auto.
+    induction q; intros; cbn in *...
+    destruct (a =? nl); inv H.
+    rewrite H2...
+  Qed.
+
+  Lemma not_inb_app_false_l: forall nl q q',
+      not_inb nl q = false ->
+      not_inb nl (q ++ q') = false.
+  Proof with auto.
+    induction q; intros; cbn in *...
+    inv H.
+    destruct (a =? nl); inv H...
+    rewrite IHq...
+  Qed.
+
+  Lemma not_inb_app_false_r: forall nl q q',
+      not_inb nl q' = false ->
+      not_inb nl (q ++ q') = false.
+  Proof with auto.
+    induction q; intros; cbn in *...
+    inv H.
+    destruct (a =? nl)... 
+    rewrite IHq...
+  Qed.
+  
+  Lemma unique_app_l: forall q q' nl n,
+      unique nl q = Some n ->
+      not_inb nl q' = true ->
+      unique nl (q ++ q') = Some n.
+  Proof with auto.
+    induction q; intros; cbn...
+    - inv H.
+    - cbn in H.
+      destruct (a =? nl).
+      destruct (not_inb nl q) eqn:Hin; inv H.
+      rewrite not_inb_app_true...
+      destruct (unique nl q) eqn:Hq.
+      + rewrite IHq with (n:=n0)...
+      + inv H.
+  Qed.
+
+  Lemma unique_last_neq: forall q t nl n,
+      (t =? nl) = false ->
+      unique nl q = Some n ->
+      unique nl (q ++ [t]) = Some n.
+  Proof with auto.
+    induction q; cbn; intros.
+    - inv H0.
+    - destruct (a =? nl) eqn:Ha...
+      + destruct (not_inb nl q) eqn:Hnl; inv H0.
+        rewrite rel_dec_correct in Ha; subst.
+        rewrite not_inb_app_true...
+        cbn.
+        now rewrite H.
+      + destruct (unique nl q) eqn:Hnl; inv H0.
+        rewrite IHq with (n:=n0)...
+  Qed.
+  Arguments unique: simpl never.
+  
   Typeclasses Transparent equ.
   Typeclasses Transparent sbisim.
-
-  Lemma sb_iter_iter: forall (k: I -> ctree E (I + R)) (x: I),
-      Ctree.iter (fun x => Ctree.map inl (Ctree.iter k x)) x ~
-        Ctree.iter (fun x =>
-    
-  Theorem rotate_agaf_pop: forall q nl,
-      <( {interp_state h_queueE rotate (q ++ [nl])}, Pure |=
-           AG AF visW {fun h => h = nl} )>.
+  Theorem rotate_agaf_pop: forall q nl i,
+      unique nl q = Some i ->
+      List.length q > 1 ->
+      <( {interp_state h_queueE rotate q}, Pure |= AG AF visW {fun h => h = nl} )>.
   Proof with eauto with ctl.
     intros.
-    eapply ag_state_iter with (R:=fun _ q _ => exists i, index q nl i).
-    - exists (List.length q).
-      apply index_last_eq.
+    unfold rotate, forever. 
+    apply ag_state_iter with
+      (R:= fun _ q _ => List.length q > 1 /\ exists i, unique nl q = Some i). 
     - constructor.
-    - clear q.
-      intros [] q w (i & Hi) Hd.
-      rewrite interp_state_bind.
-      setoid_rewrite (@interp_state_trigger _ _ _ _ _ _ Pop _); cbn.
-      rewrite bind_bind.
-      setoid_rewrite sb_guard.
-      setoid_rewrite bind_ret_l.
-      destruct q.
-      + inv Hi.
-      + rewrite bind_bind.
+    - split... 
+    - clear H H0 q i.
+      intros [] q w Hd (Hlen & i & Hi).
+      split.
+      + (* Eventually *)
+        eapply aul_state_iter_nat with
+          (Ri:= fun _ q _ => List.length q > 1 /\ exists i, unique nl q = Some i)
+          (f:= fun 'tt q (w: WorldW T) =>
+                 match unique nl q with
+                 | Some n => 1 + List.length q - n
+                 | None => List.length q
+                 end)...
+        * clear Hlen Hi q w Hd i.
+          intros [] q w Hd (Hlen & i & Hi).
+          rewrite interp_state_map, ctlr_map, ctll_map, interp_state_bind; cbn...
+          setoid_rewrite (@interp_state_trigger _ _ _ _ _ _ Pop _); cbn.
+          rewrite bind_bind.
+          setoid_rewrite sb_guard.
+          setoid_rewrite bind_ret_l.
+          destruct q.
+          -- (* q' = nl :: ts *)
+            left.
+            inv Hi.
+          -- (* q' = h :: ts, index ts nl n *)
+            right.
+            rewrite bind_bind.
+            eapply aur_bind_r_eq.
+            ++ eapply aur_vis...
+               right; split.
+               ** csplit...
+               ** intros [].
+                  cleft.
+                  apply anr_ret...
+            ++ rewrite bind_ret_l.
+               rewrite interp_state_bind.
+               setoid_rewrite (@interp_state_trigger _ _ _ _ _ _ (Push t) _);
+                 simpl runStateT.
+               rewrite bind_bind, bind_ret_l, sb_guard, bind_ret_l,
+                 interp_state_ret.
+               cleft.
+               apply anr_ret...
+               exists tt; intuition.
+               ** rewrite app_length.
+                  cbn in *.
+                  lia.
+               ** cbn in Hi; destruct (t =? nl) eqn:Hnl;
+                    destruct (not_inb nl q) eqn:Hinb; inv Hi...
+                  --- (* t = nl, nl not in q *)
+                    apply rel_dec_correct in Hnl; subst.
+                    exists (List.length q).
+                    now apply unique_last_eq.
+                  --- (* t = nl, nl in q *)
+                    apply rel_dec_correct in Hnl; subst.
+                    unfold unique in H0; cbn in H0.
+                    rewrite rel_dec_eq_true in H0...
+                    rewrite Hinb in H0; inv H0.
+                  --- (* t <> nl, nl not in q *)
+                    apply not_inb_unique_none in Hinb.
+                    apply unique_head_neq in H0...
+                    rewrite Hinb in H0; inv H0.
+                  --- (* t <> nl, nl in q *)
+                    apply unique_head_neq in H0...
+                    exists (i - 1).
+                    apply unique_app_l; auto.
+                    cbn; now rewrite Hnl.
+               ** cbn in *.
+                  destruct (t =? nl) eqn:Hnl.
+                  --- (* t = nl *)
+                    apply unique_head_eq in Hi...
+                    rewrite rel_dec_correct in Hnl; subst.
+                    rewrite unique_last_eq...
+                    rewrite unique_head_eq'...
+                    destruct (length q) eqn:Hl; try lia.
+                    rewrite app_length; cbn.
+                    rewrite Hl; cbn.
+                    destruct n; lia.
+                  --- (* t <> nl *)
+                    rewrite unfold_unique_hd, Hnl in Hi.
+                    destruct (unique nl q) eqn:Hnl'; inv Hi.
+                    rewrite unique_last_neq with (n:=n)...
+                    rewrite unfold_unique_hd, Hnl, Hnl'.
+                    rewrite app_length.
+                    cbn; destruct n.
+      + (* Loop invariant *)
+        rewrite interp_state_map, ctlr_map, interp_state_bind,
+          (@interp_state_trigger _ _ _ _ _ _ Pop _), bind_bind; cbn...
+        setoid_rewrite sb_guard.
         setoid_rewrite bind_ret_l.
-        unfold log, trigger.
-        (* Without this it's impossible to prove *)
-        rewrite bind_vis.
-        eapply axr_vis...
-        split.
-        * eapply afl_vis...
-          right.
-          split...
-          intros [].
-          rewrite bind_ret_l.
-          rewrite interp_state_bind, interp_state_vis, bind_bind.
-          cbn.
-          rewrite bind_ret_l, sb_guard, interp_state_ret, bind_ret_l,
-            interp_state_ret.          
-          dependent induction Hi. 
-          -- cleft.
-             csplit...
-          -- admit.
-        * intros [].
-          rewrite bind_ret_l, interp_state_bind, interp_state_vis.
-          cbn.
-          rewrite bind_bind, bind_ret_l, sb_guard, interp_state_ret,
-            bind_ret_l, interp_state_ret.
-          cleft.
-          apply anr_ret...
-          exists tt; split2...
-          exists (List.length q).
-          admit.
+        destruct q; cbn in Hlen; try lia.
+        rewrite unfold_unique_hd in Hi.
+        destruct (t =? nl) eqn:Ht.
+        destruct (not_inb nl q) eqn:Hinb; inv Hi.
+        * (* q = nl :: ts *)
+          rewrite bind_bind.
+          unfold log, trigger.
+          rewrite bind_vis.
+          apply axr_vis...
+          split.
+          -- csplit...
+          -- intros [].
+             rewrite ?bind_ret_l.
+             rewrite interp_state_bind, interp_state_vis, bind_bind.
+             cbn.
+             rewrite bind_ret_l, sb_guard, interp_state_ret, bind_ret_l,
+               interp_state_ret.
+             cleft.
+             apply anr_ret...
+             exists tt; intuition.
+             ++ rewrite app_length; cbn; lia.
+             ++ exists (List.length q).
+                rewrite rel_dec_correct in Ht; subst.
+                now apply unique_last_eq.
+        * (* q = h :: ts *)          
+          rewrite bind_bind.
+          unfold log, trigger.
+          rewrite bind_vis.
+          apply axr_vis...
+          split.
+          -- csplit...
+          -- intros [].
+             rewrite ?bind_ret_l.
+             rewrite interp_state_bind, interp_state_vis, bind_bind.
+             cbn.
+             rewrite bind_ret_l, sb_guard, interp_state_ret, bind_ret_l,
+               interp_state_ret.
+             cleft.
+             apply anr_ret...
+             exists tt; intuition.
+             ++ rewrite app_length; cbn; lia.
+             ++ destruct (unique nl q) eqn:Hnl; inv Hi.
+                exists n.
+                now apply unique_last_neq...
   Admitted.
 End QueueEx.
   
