theories/CTree/Logic/Iter.v
@@ -1,11 +1,12 @@
 From Coinduction Require Import
-  coinduction lattice.
+  coinduction lattice tactics.
 
 From CTree Require Import
   Events.Core
   CTree.Core
   CTree.Equ
   CTree.SBisim
+  CTree.Eq.Bind
   CTree.Logic.Trans
   CTree.Logic.CanStep
   CTree.Logic.AX
@@ -16,6 +17,8 @@ From CTree Require Import
   CTree.Logic.Bind
   CTree.Logic.Ret
   Logic.Ctl.
+
+From Coq Require Import Arith.Wf_nat.
 
 Generalizable All Variables.
 
@@ -177,10 +180,11 @@ Section IterLemmas.
     rename H into HindWf.
     intros.
     unfold iter, MonadIter_ctree.
-    rewrite unfold_iter.
     destruct (H _ _ Hi).
-    - now eapply ctll_bind_l.
-    - eapply aul_bind_r with
+    - rewrite unfold_iter.
+      apply ctll_bind_l... 
+    - rewrite unfold_iter.
+      eapply aul_bind_r with
         (R:=fun (lr: I + X) (w': World E) =>
               exists i' : I, lr = inl i' /\ Ri i' w' /\ Rv (i', w') (i, w))... 
       intros [i' | r] w'.            
@@ -193,6 +197,22 @@ Section IterLemmas.
       + intros (j & Hcontra & ?); inv Hcontra.
   Qed.
 
+  Lemma aul_iter_nat{X I} Ri (f: I -> World E -> nat) (i: I) w (k: I -> ctree E (I + X))
+    (φ ψ: ctll E):
+    Ri i w ->    
+    (forall (i: I) w,
+        Ri i w ->
+        <( {k i}, w |= φ AU ψ )> \/
+          <[ {k i}, w |= φ AU AN done
+                      {fun (lr: I + X) (w': World E) =>
+                         exists i', lr = inl i' /\ Ri i' w' /\ f i'  w' < f i w}]>) ->
+    <( {iter k i}, w |= φ AU ψ )>.
+  Proof.
+    intros.
+    eapply aul_iter with Ri (ltof _ (fun '(i, w) => f i w)); auto.
+    apply well_founded_ltof.
+  Qed.
+  
   Lemma aur_iter{X I} Ri (Rv: relation (I * World E)) (i: I) w (k: I -> ctree E (I + X)) (φ: ctll E) (ψ: ctlr E X):
     well_founded Rv ->
     Ri i w ->    
@@ -234,6 +254,23 @@ Section IterLemmas.
     - apply aur_ret.
   Qed.
 
+  Lemma aur_iter_nat{X I} Ri (f: I -> World E -> nat) (i: I) w (k: I -> ctree E (I + X)) (φ: ctll E) (ψ: ctlr E X):
+    Ri i w ->    
+    (forall (i: I) w,
+        Ri i w ->
+        <[ {k i}, w |= φ AU AN done
+                    {fun (lr: I + X) (w': World E) =>
+                       match lr with
+                       | inl i' => Ri i' w' /\ f i' w' < f i w
+                       | inr r => <[ {Ret r}, w' |= ψ \/ φ AX ψ ]>
+                       end} ]>) ->
+    <[ {iter k i}, w |= φ AU ψ ]>.
+  Proof.
+    intros.
+    eapply aur_iter with Ri (ltof _ (fun '(i, w) => f i w)); auto.
+    apply well_founded_ltof.
+  Qed.
+  
   (* EU *)
   Lemma eul_iter{X I} Ri (Rv: relation (I * World E)) (i: I) w (k: I -> ctree E (I + X)) (φ ψ: ctll E):
     well_founded Rv ->
@@ -316,31 +353,33 @@ Section IterLemmas.
   
   (* AG *)
   Typeclasses Transparent sbisim.
-  Lemma ag_iter{X I} R (i: I) w (k: I -> ctree E (I + X)) (φ: ctll E) (ψ: ctlr E X):
-    R i w ->    
+  Lemma ag_iter{X I} (R: rel I (World E)) (i: I) w (k: I -> ctree E (I + X)) φ:
+    R i w ->
     (forall (i: I) w,
         R i w ->
-        <[ {k i}, w |= φ AX (φ AU AN done
-                    {fun (lr: I + X) (w': World E) =>
-                       exists (i': I), lr = inl i' /\ R i' w'}) ]>) ->
+        <( {iter k i}, w |= φ)> /\
+          <[ {k i}, w |= AN (φ AU AN done
+                      {fun (lr: I + X) (w': World E) =>
+                         exists (i': I), lr = inl i' /\ R i' w'}) ]>) ->
     <( {iter k i}, w |= AG φ )>.
   Proof with auto with ctl.
-    intros.
+    intros HR H.
     (* coinductive case *)
     generalize dependent i.
     generalize dependent w.
     unfold iter, MonadIter_ctree.
-    setoid_rewrite sb_unfold_iter.
     coinduction RR CIH; intros.
-    specialize (H0 _ _ H) as H0'.
-    cdestruct H0'.
+    specialize (H _ _ HR) as (Hφ & H').
+    cdestruct H'.
     split2.
-    - now apply ctll_bind_l.
-    - destruct Hs as (k' & wk & TRk).
+    - apply Hφ. 
+    - destruct Hs as (k' & wk & TR).
+      rewrite unfold_iter.
       apply can_step_bind_l with k' wk...
-      specialize (H0' _ _ TRk).
-      now apply aur_not_done in H0'.
+      specialize (H' _ _ TR).
+      now apply aur_not_done in H'.
     - intros t' w' TR.
+      rewrite unfold_iter in TR.
       apply ktrans_bind_inv in TR as
           [(t0' & TR0 & Hd_ & Heq) | (x' & w0 & TRt0 & Hd & TRk)].
       + (* [k x] steps *)
@@ -348,21 +387,22 @@ Section IterLemmas.
         apply (ft_t (ag_bind_ag φ
                        (fun (lr: I+X) (w0: World E) => exists i' : I, lr = inl i' /\ R i' w0))).
         apply in_bind_ctx1.
-        * now apply H0'. 
-        * intros [l | r] w_ (? & Hinv & HR); inv Hinv.
-          rewrite sb_unfold_iter.
+        * now apply H'. 
+        * intros [l | r] w_ (? & Hinv & HR'); inv Hinv.
+          rewrite sb_guard. 
           apply CIH...
       + (* [k x] returns *)        
-        specialize (H0' _ _ TRt0) as HAX.
+        specialize (H' _ _ TRt0) as HAX.
         now apply aur_stuck, axr_stuck in HAX.
-  Qed.
+  Qed.        
 
   (* EG *)
-  Lemma eg_iter{X I} R (i: I) w (k: I -> ctree E (I + X)) (φ: ctll E) (ψ: ctlr E X):
+  Lemma eg_iter{X I} R (i: I) w (k: I -> ctree E (I + X)) (φ: ctll E):
     R i w ->    
     (forall (i: I) w,
         R i w ->
-        <[ {k i}, w |= φ EX (φ EU EN done
+        <( {iter k i}, w |= φ)> /\
+        <[ {k i}, w |= EN (φ EU EN done
                     {fun (lr: I + X) (w': World E) =>
                        exists (i': I), lr = inl i' /\ R i' w'}) ]>) ->
     <( {iter k i}, w |= EG φ )>.
@@ -372,24 +412,25 @@ Section IterLemmas.
     generalize dependent i.
     generalize dependent w.
     unfold iter, MonadIter_ctree.
-    setoid_rewrite sb_unfold_iter.
     coinduction RR CIH; intros.
-    specialize (H0 _ _ H) as H0'.
+    specialize (H0 _ _ H) as (Hφ & H0').
     cdestruct H0'.
     split.
-    - now apply ctll_bind_l.
+    - apply Hφ. 
     - exists (lr <- t;; match lr with
-                 | inl l => Ctree.iter k l
+                 | inl l => Guard (Ctree.iter k l)
                  | inr r => Ret r
                   end), w0; split.
-      + apply ktrans_bind_r...
+      + rewrite unfold_iter.
+        apply ktrans_bind_r...
         now apply eur_not_done in H0'.
       + apply (ft_t (eg_bind_eg φ
                        (fun (lr: I+X) (w0: World E) => exists i' : I, lr = inl i' /\ R i' w0))).
         apply in_bind_ctx1.
         * now apply H0'. 
-        * intros [l | r] w_ (? & Hinv & HR); inv Hinv.
-          rewrite sb_unfold_iter.
+        * intros [l | r] w_ (? & Hinv & HR); inv Hinv.          
+          rewrite sb_guard.
           apply CIH...
   Qed.
+
 End IterLemmas.
