theories/Logic/Ctl.v
@@ -3,10 +3,11 @@
 Modal logics over ctrees
 =========================================
 |*)
-From Coinduction Require Export coinduction.
+From Coinduction Require Export coinduction tactics.
 From CTree Require Export           
   Utils.Utils
   Logic.Kripke
+  Logic.Syntax
   Logic.Semantics
   Logic.Congruence
   Logic.Setoid
